Fir/Wasm/Concrete.lean
@@ -11,3 +11,4 @@ import Fir.Wasm.Concrete.HeapRefinement
 import Fir.Wasm.Concrete.ConstructorAllocationCorrectness
 import Fir.Wasm.Concrete.ConstructorHeapCorrectness
 import Fir.Wasm.Concrete.ProjectionCorrectness
+import Fir.Wasm.Concrete.TagMutationCorrectness
